concurrency/common/ClightSemanticsForMachines.v
@@ -17,11 +17,14 @@ Require Import List. Import ListNotations.
 
 (* The concurrent machinery*)
 (*Require Import VST.concurrency.common.core_semantics.*)
+Require Import VST.sepcomp.mem_lemmas.
+Require Import VST.concurrency.memsem_lemmas.
 Require Import VST.concurrency.common.scheduler.
 Require Import VST.concurrency.common.HybridMachineSig.
 Require Import VST.concurrency.common.semantics.
 Require Import VST.concurrency.common.lksize.
 Require Import VST.concurrency.common.permissions.
+Require Import VST.concurrency.common.dry_machine_lemmas.
 
 Import Ctypes. 
 Require Import compcert.cfrontend.Clight.
@@ -30,18 +33,84 @@ Arguments sizeof {env} !t / .
 
 (*Semantics*)
 Require Import VST.veric.Clight_core.
-Require Import VST.veric.Clightcore_coop. 
+Require Import VST.veric.Clightcore_coop.
 Require Import VST.sepcomp.event_semantics.
 Require Import VST.veric.Clight_evsem.
 
-  Lemma at_external_SEM_eq:
-     forall ge c m, semantics.at_external (CLC_evsem ge) c m =
-     match c with
-     | Callstate (External ef _ _ _) args _ => 
-         if ef_inline ef then None else Some (ef, args)
-     | _ => None
-   end.
-  Proof. auto. Qed.
+Set Bullet Behavior "Strict Subproofs".
 
-  #[export] Instance ClightSem ge : Semantics :=
-    { semG := G; semC := C; semSem := CLC_evsem ge; the_ge := ge }.
+Lemma at_external_SEM_eq:
+   forall ge c m, semantics.at_external (CLC_evsem ge) c m =
+   match c with
+   | Callstate (External ef _ _ _) args _ => 
+       if ef_inline ef then None else Some (ef, args)
+   | _ => None
+ end.
+Proof. auto. Qed.
+
+#[export] Instance ClightSem ge : Semantics :=
+  { semG := G; semC := C; semSem := CLC_evsem ge; the_ge := ge }.
+
+Lemma CLC_step_decay: forall g c m tr c' m',
+      event_semantics.ev_step (CLC_evsem g) c m tr c' m' ->
+      decay m m'.
+Proof.
+intros.
+pose proof (msem_decay (CLC_memsem g) c m c' m').
+apply H0. clear H0.
+simpl in *.
+apply CLC_evstep_ax1 in H.
+auto.
+Qed.
+
+#[export] Instance ClightAxioms ge : @CoreLanguage.SemAxioms (ClightSem ge).
+Proof.
+  constructor.
+  - intros.
+    apply mem_step_obeys_cur_write; auto.
+    eapply corestep_mem; eauto.
+  - intros.
+    apply ev_step_ax2 in H as [].
+    eapply CLC_step_decay; simpl in *; eauto.
+  - intros.
+    apply mem_forward_nextblock, mem_step_forward.
+    eapply corestep_mem; eauto.
+  - intros; simpl.
+    destruct q; auto.
+  - intros.
+    destruct Hstep as (? & ->); done. (* Do we need initial_core to allocate the arguments? *)
+(*    inv Hstep.
+    inv H; simpl.
+    apply mem_step_obeys_cur_write; auto.
+  (* apply memsem_lemmas.mem_step_refl. *)
+    eapply mem_step_alloc; eauto. *)
+  - intros.
+    destruct H as (? & ->).
+    apply strong_decay_refl.
+(*    inv H.
+    inv H0; simpl.
+    split; intros.
+    + (*contradiction. *)
+      eapply juicy_mem.fullempty_after_alloc in H8.
+      admit. 
+      (* destruct H8; [right|left].
+     
+       should be able to prove that 
+                1. b = Mem.nextblock m
+                which satisfies the goal at all offsets.
+              *)
+        
+    + auto. inv H8.
+      simpl.
+      Transparent Mem.alloc.
+      unfold Mem.alloc; simpl.
+      admit.
+      
+  - intros.
+    inv H.
+    inv H0; simpl.
+    erewrite (Mem.nextblock_alloc _ _ _ _ _ H8).
+    xomega.*)
+  - intros.
+    destruct H as (? & ->); done.
+Qed.
